
\documentclass[a4paper,12pt]{article}
%%%%%%%%%%%%%%%%%%%%%%%%%%%%%%%%%%%%%%%%%%%%%%%%%%%%%%%%%%%%%%%%%%%%%%%%%%%%%%%%%%%%%%%%%%%%%%%%%%%%%%%%%%%%%%%%%%%%%%%%%%%%%%%%%%%%%%%%%%%%%%%%%%%%%%%%%%%%%%%%%%%%%%%%%%%%%%%%%%%%%%%%%%%%%%%%%%%%%%%%%%%%%%%%%%%%%%%%%%%%%%%%%%%%%%%%%%%%%%%%%%%%%%%%%%%%
\usepackage{amssymb}
\usepackage{amsfonts}
\usepackage{graphicx}
\usepackage{amsmath}

\setcounter{MaxMatrixCols}{10}
%TCIDATA{OutputFilter=LATEX.DLL}
%TCIDATA{Version=5.50.0.2953}
%TCIDATA{<META NAME="SaveForMode" CONTENT="1">}
%TCIDATA{BibliographyScheme=Manual}
%TCIDATA{Created=Sat Oct 14 01:01:49 2006}
%TCIDATA{LastRevised=Sunday, August 08, 2021 22:41:09}
%TCIDATA{<META NAME="GraphicsSave" CONTENT="32">}
%TCIDATA{<META NAME="DocumentShell" CONTENT="Journal Articles\Standard LaTeX Article">}
%TCIDATA{CSTFile=LaTeX article (bright).cst}

\textheight=26.5cm
\textwidth=18cm
\oddsidemargin=-1.0cm
\evensidemargin=-1.0cm
\topmargin=-2.5cm
\def\baselinestretch{1.6}
\input{tcilatex}
\begin{document}


;

\subsection{separa\c{c}\~{a}o de vari\'{a}veis - corrigido}

;%
\begin{eqnarray*}
\nabla ^{2}u &=&\frac{1}{a^{2}\left( \sinh ^{2}\chi +\cos ^{2}\theta
_{2}\right) }\left[ \frac{1}{\sin \theta _{2}}\frac{\partial }{\partial
\theta _{2}}\left( \sin \theta _{2}\frac{\partial u}{\partial \theta _{2}}%
\right) +\frac{1}{\cosh \chi }\frac{\partial }{\partial \chi }\left( \cosh
\chi \frac{\partial u}{\partial \chi }\right) \right]  \\
&&+\frac{1}{a^{2}\sin ^{2}\theta _{2}\cosh ^{2}\chi }\frac{\partial ^{2}u}{%
\partial \theta _{1}^{2}}
\end{eqnarray*}%
\begin{equation*}
u\left( \theta _{1},\theta _{2},\chi \right) =y_{1}\left( \theta _{1}\right)
W\left( \theta _{2},\chi \right) 
\end{equation*}%
\begin{equation*}
\frac{\sin ^{2}\theta _{2}\cosh ^{2}\chi }{\left( \sinh ^{2}\chi +\cos
^{2}\theta _{2}\right) }\left[ \frac{1}{\sin \theta _{2}}\frac{\partial }{%
\partial \theta _{2}}\left( \sin \theta _{2}\frac{\partial W}{\partial
\theta _{2}}\right) +\frac{1}{\cosh \chi }\frac{\partial }{\partial \chi }%
\left( \cosh \chi \frac{\partial W}{\partial \chi }\right) \right] y_{1}=-W%
\frac{\partial ^{2}u}{\partial \theta _{1}^{2}}
\end{equation*}%
\begin{equation*}
\frac{1}{W}\frac{\sin ^{2}\theta _{2}\cosh ^{2}\chi }{\left( \sinh ^{2}\chi
+\cos ^{2}\theta _{2}\right) }\left[ \frac{1}{\sin \theta _{2}}\frac{%
\partial }{\partial \theta _{2}}\left( \sin \theta _{2}\frac{\partial W}{%
\partial \theta _{2}}\right) +\frac{1}{\cosh \chi }\frac{\partial }{\partial
\chi }\left( \cosh \chi \frac{\partial W}{\partial \chi }\right) \right] =-%
\frac{1}{y_{1}}\frac{d^{2}y_{1}}{d\theta _{1}^{2}}=\lambda _{1}
\end{equation*}%
\begin{equation*}
\frac{d^{2}y_{1}}{d\theta _{1}^{2}}+\lambda _{1}y_{1}=0,\ y_{1}\left( \theta
_{1}\right) =y_{1}\left( \theta _{1}+2\pi \right) 
\end{equation*}%
a%
\begin{equation*}
\left[ \frac{1}{\sin \theta _{2}}\frac{\partial }{\partial \theta _{2}}%
\left( \sin \theta _{2}\frac{\partial W}{\partial \theta _{2}}\right) +\frac{%
1}{\cosh \chi }\frac{\partial }{\partial \chi }\left( \cosh \chi \frac{%
\partial W}{\partial \chi }\right) \right] =\frac{\left( \sinh ^{2}\chi
+\cos ^{2}\theta _{2}\right) }{\sin ^{2}\theta _{2}\cosh ^{2}\chi }\lambda
_{1}W
\end{equation*}%
\begin{equation*}
\cosh ^{2}\chi -\sinh ^{2}\chi =1,\ \cos ^{2}\theta _{2}+\sin ^{2}\theta
_{2}=1
\end{equation*}%
\begin{equation*}
\left( \sinh ^{2}\chi +\cos ^{2}\theta _{2}\right) =\left( \sinh ^{2}\chi
+1+\cos ^{2}\theta _{2}-1\right) =\cosh ^{2}\chi -\sin ^{2}\theta _{2}
\end{equation*}%
p%
\begin{equation*}
\frac{\left( \sinh ^{2}\chi +\cos ^{2}\theta _{2}\right) }{\sin ^{2}\theta
_{2}\cosh ^{2}\chi }=\frac{\cosh ^{2}\chi -\sin ^{2}\theta _{2}}{\sin
^{2}\theta _{2}\cosh ^{2}\chi }=\frac{1}{\sin ^{2}\theta _{2}}-\frac{1}{%
\cosh ^{2}\chi }
\end{equation*}%
p%
\begin{equation*}
\left[ \frac{1}{\sin \theta _{2}}\frac{\partial }{\partial \theta _{2}}%
\left( \sin \theta _{2}\frac{\partial W}{\partial \theta _{2}}\right) +\frac{%
1}{\cosh \chi }\frac{\partial }{\partial \chi }\left( \cosh \chi \frac{%
\partial W}{\partial \chi }\right) \right] =\lambda _{1}W\left( \frac{1}{%
\sin ^{2}\theta _{2}}-\frac{1}{\cosh ^{2}\chi }\right) 
\end{equation*}%
\begin{equation*}
W\left( \theta _{2},\chi \right) =y_{2}\left( \theta _{2}\right) Z\left(
\chi \right) 
\end{equation*}%
\begin{equation*}
\left[ \frac{1}{\sin \theta _{2}}\frac{d}{d\theta _{2}}\left( \sin \theta
_{2}\frac{dy_{2}}{d\theta _{2}}\right) Z+\frac{1}{\cosh \chi }\frac{d}{d\chi 
}\left( \cosh \chi \frac{dZ}{d\chi }\right) y_{2}\right] =\lambda
_{1}y_{2}Z\left( \frac{1}{\sin ^{2}\theta _{2}}-\frac{1}{\cosh ^{2}\chi }%
\right) 
\end{equation*}%
\begin{equation*}
\frac{1}{y_{2}}\frac{1}{\sin \theta _{2}}\frac{d}{d\theta _{2}}\left( \sin
\theta _{2}\frac{dy_{2}}{d\theta _{2}}\right) +\frac{1}{Z}\frac{1}{\cosh
\chi }\frac{d}{d\chi }\left( \cosh \chi \frac{dZ}{d\chi }\right) =\lambda
_{1}\left( \frac{1}{\sin ^{2}\theta _{2}}-\frac{1}{\cosh ^{2}\chi }\right) 
\end{equation*}%
\begin{equation*}
\frac{1}{y_{2}}\frac{1}{\sin \theta _{2}}\frac{d}{d\theta _{2}}\left( \sin
\theta _{2}\frac{dy_{2}}{d\theta _{2}}\right) -\frac{\lambda _{1}}{\sin
^{2}\theta _{2}}=-\frac{1}{Z}\frac{1}{\cosh \chi }\frac{d}{d\chi }\left(
\cosh \chi \frac{dZ}{d\chi }\right) +\left( -\frac{\lambda _{1}}{\cosh
^{2}\chi }\right) =-\lambda _{2}
\end{equation*}%
p obtemos 3 eq dif ordinarias%
\begin{equation*}
\frac{1}{\sin \theta _{2}}\frac{d}{d\theta _{2}}\left( \sin \theta _{2}\frac{%
dy_{2}}{d\theta _{2}}\right) +\left( \lambda _{2}-\frac{\lambda _{1}}{\sin
^{2}\theta _{2}}\right) y_{2}=0
\end{equation*}%
\begin{equation*}
\frac{1}{\cosh \chi }\frac{d}{d\chi }\left( \cosh \chi \frac{dZ}{d\chi }%
\right) +\left( -\lambda _{2}+\frac{\lambda _{1}}{\cosh ^{2}\chi }\right) Z=0
\end{equation*}%
\begin{equation*}
\frac{d^{2}y_{1}}{d\theta _{1}^{2}}+\lambda _{1}y_{1}=0,\ y_{1}\left( \theta
_{1}\right) =y_{1}\left( \theta _{1}+2\pi \right) 
\end{equation*}%
;

\end{document}
